chore: Remove redundant postconditions
Many of the postconditions of `GetEncryptionMaterials` and `DecryptMaterials`
followed from the validity of the output parameter. In turn, the validity of the
output parameter follows from its `Valid...` type.

In the case of `GetEncryptionMaterials`, two of the postconditions were
conveniently captured into a new member function `EncryptionMaterials.Serializable`
(which is a predicate that is also needed in Caching CMM).

src/SDK/Materials.dfy
@@ -84,8 +84,11 @@ module {:extern "Materials"} Materials {
       && GenerateTraceEntriesConsistent(plaintextDataKey, keyringTrace)
       && |Filter(keyringTrace, IsEncryptTraceEntry)| == |encryptedDataKeys|
       // TODO: Strongly tie each trace entry to it's corresponding EDK (https://github.com/awslabs/aws-encryption-sdk-dafny/issues/100)
-//      && |encryptedDataKeys| > 0 // KRML new
-//      && Context.ValidAAD(encryptionContext) // KRML new
+    }
+
+    predicate Serializable() {
+      && |encryptedDataKeys| > 0
+      && EncryptionContext.Serializable(encryptionContext)
     }
 
     static function method ValidWitness(): EncryptionMaterials {
